Updated the Coq files with a very broken insert.

code/bplustree.v
@@ -1,19 +1,40 @@
 Require Export SfLib.
 
+Definition blt_nat (n m : nat) : bool :=
+  ble_nat (S n) m.
 
 Inductive bplustree (b: nat) (X:Type) : Type :=
-  | bptNode : list (nat * (bplustree b X)) -> bplustree b X -> bplustree b X
+  | bptNode : bplustree b X -> list (nat * (bplustree b X)) -> bplustree b X
   | bptLeaf : list (nat * X) -> bplustree b X
   . 
 
 
 Example test := bptLeaf 2 bool [(1, true), (2, false)].
 
-Definition left := bptLeaf 2 nat [(4, 4), (5, 5)].
-Definition centre := bptLeaf 2 nat [(7, 7)].
-Definition right := bptLeaf 2 nat [(9, 9)].
-Definition root := bptNode 2 nat [(6, left), (8, centre)] right.
 
+Definition head {X: Type} {b: nat} (kpl: (list (nat * bplustree b X))) : option nat :=
+  match kpl with
+    | nil => None
+    | (k, v) :: kvl' => Some k
+  end.
+  
+Definition peek {X: Type} {b: nat} (tree: (bplustree b X)) : nat :=
+  match tree with
+    | bptLeaf kvl => match kvl with
+      | nil => 0
+      | (k,v) :: kvl' => k
+      end
+    | bptNode sp kpl => match head kpl with
+      | Some k => k
+      | None => 0
+      end
+  end. 
+
+
+Definition left := bptLeaf 2 nat [(4, 44), (5, 55)].
+Definition centre := bptLeaf 2 nat [(7, 77)].
+Definition right := bptLeaf 2 nat [(9, 99)].
+Definition root := bptNode 2 nat left [(peek centre, centre), (peek right, right)].
 
 Fixpoint search_leaf {X: Type} (sk: nat) (kvl: (list (nat * X))) : option X :=
   match kvl with
@@ -21,33 +42,141 @@ Fixpoint search_leaf {X: Type} (sk: nat) (kvl: (list (nat * X))) : option X :=
     | (k, v) :: kvl' => if beq_nat k sk then Some v else search_leaf sk kvl'
   end.
 
+Fixpoint find_child {X: Type} {b: nat} (sk: nat) (sp: (bplustree b X)) (kpl: (list (nat * bplustree b X))) : option (bplustree b X) :=
+  let fix find_child' (kpl: (list (nat * bplustree b X))) : option (bplustree b X) :=
+    match kpl with
+      | nil => None
+      | (k, p) :: kpl' => match head kpl' with
+        | None => Some p
+        | Some k' => if andb (ble_nat k sk) (blt_nat sk k')
+      						then Some p
+      						else find_child' kpl'
+       end
+     end 
+  in 
+  match head kpl with
+    | None => None
+    | Some k => if blt_nat sk k
+      then Some sp
+      else find_child' kpl
+  end.
+
 Fixpoint search {X: Type} {b: nat} (sk: nat) (tree: (bplustree b X)) : option X :=
   let fix search_node
                       (kpl: (list (nat * bplustree b X)))
-                   : option (option X) :=
+                   : option X :=
     match kpl with
       | nil => None
-      | (k, p) :: kpl' => if ble_nat sk k then Some (search sk p) else search_node kpl'
-    end
+      | (k, p) :: kpl' => match head kpl' with
+        | None => search sk p
+        | Some k' => if andb (ble_nat k sk) (blt_nat sk k')
+      						then search sk p
+      						else search_node kpl'
+       end
+     end 
   in 
   match tree with
     | bptLeaf kvl => search_leaf sk kvl
-    | bptNode kpl ep => match search_node kpl with
-      | Some k => k
-      | None => search sk ep
+    | bptNode sp kpl => match head kpl with
+      | None => None
+      | Some k => if blt_nat sk k
+      	then search sk sp
+      	else search_node kpl
     end
   end.
 
 
-Example search_test_find_item_left : search 4 root = Some 4.
+Example search_test_find_item_left : search 4 root = Some 44.
 Proof. simpl. reflexivity. Qed.
-Example search_test_find_item_centre : search 7 root = Some 7.
+Example search_test_find_item_centre : search 7 root = Some 77.
 Proof. simpl. reflexivity. Qed.
-Example search_test_find_item_right : search 9 root = Some 9.
+Example search_test_find_item_right : search 9 root = Some 99.
 Proof. simpl. reflexivity. Qed.
 Example search_test_cant_find_missing : search 6 root = None.
 Proof. simpl. reflexivity. Qed.
 
 
+Fixpoint insert_into_list {X: Type} (k: nat) (v: X) (kvl: list (nat * X)) : list (nat * X) :=
+  match kvl with 
+    | nil => [(k, v)]
+    | (k', v') :: kvl' => if ble_nat k k'
+    						then if beq_nat k k' then ((k, v) :: kvl') else ((k, v) :: kvl)
+    						else (k', v') :: (insert_into_list k v kvl')
+  end.
 
+Fixpoint split_list' {X: Type} (b: nat) (fst snd: list X) : (list X * list X) :=
+  match b with
+    | O => (rev fst, snd)
+    | S b' => match snd with
+      | nil => (rev fst, snd)
+      | f::snd' => split_list' b' (f::fst) snd'
+    end
+  end. 
+Definition split_list {X: Type} (b: nat) (lst: list X) : (list X * list X) :=
+  split_list' b [] lst.
+
+Definition insert_leaf {X: Type} (b: nat) (k: nat) (v: X) (kvl: list (nat * X))
+						: (list (nat * X) * option (list (nat * X))) :=
+  let
+  	kvl' := insert_into_list k v kvl
+  in
+    if ble_nat (length kvl') (mult b 2)
+      then (kvl', None)
+      else let (fst, snd) := split_list b kvl' in (fst, Some snd) 
+  .
+  
+(*  
+Fixpoint insert {X: Type} {b: nat} (sk: nat) (v: X) (tree: (bplustree b X))
+              : (bplustree b X * option (bplustree b X)) := 
+  match tree with
+    | bptLeaf kvl => let (fst, snd_opt) := insert_leaf b sk v kvl in
+                     match snd_opt with
+                       | None => (bptLeaf b X fst, None)
+                       | Some snd => (bptLeaf b X fst, Some (bptLeaf b X snd))
+                     end
+    | bptNode sp kpl => match find_child sk sp kpl with
+      | None => (tree, None)
+      | Some p => insert sk v p
+    end
+  end.
+*)
+  
+Fixpoint insert {X: Type} {b: nat} (sk: nat) (v: X) (tree: (bplustree b X))
+                : (bplustree b X * option (bplustree b X)) :=
+
+  (* More or less copy-pasted from search *)
+  let fix split_if_necessary (input: (bplustree b X * option (bplustree b X)))
+  							: (bplustree b X * option (bplustree b X)) :=
+  							match input with
+  							  | (tree, None) => (tree, None)
+  							  | (tree, Some new) => (tree, Some new)
+  							end
+  in 
+  let fix insert_into_node
+                      (kpl: (list (nat * bplustree b X)))
+                   : (bplustree b X * option (bplustree b X)) :=
+    match kpl with
+      | nil => (tree, None)
+      | (k, p) :: kpl' => match head kpl' with
+        | None => split_if_necessary (insert k v p)
+        | Some k' => if andb (ble_nat k sk) (blt_nat sk k')
+      						then split_if_necessary (insert k v p)
+      						else insert_into_node kpl'
+       end
+     end 
+     
+  in 
+  match tree with
+    | bptLeaf kvl => let (fst, snd_opt) := insert_leaf b sk v kvl in
+                     match snd_opt with
+                       | None => (bptLeaf b X fst, None)
+                       | Some snd => (bptLeaf b X fst, Some (bptLeaf b X snd))
+                     end 
+    | bptNode sp kpl => match head kpl with
+      | None => (tree, None)
+      | Some k => if blt_nat sk k
+      	then split_if_necessary (insert k v sp)
+      	else insert_into_node kpl
+    end
+  end.
   
